Experiment with soundly modeling expression evaluation order

src/program_proof/controlflow/x.v
@@ -1,16 +1,6 @@
 From Perennial.goose_lang Require Import prelude.
 From Perennial.goose_lang Require Import ffi.grove_prelude.
-
-Definition do_return : expr.
-Admitted.
-
-Definition test : val :=
-  λ: <>,
-     (if: (#0 = #0) then
-       do_return #3
-      else #()) ;;
-    do_return #2
-.
+From Goose Require sync. Module mysync := sync.
 
 Definition returnV: val := #str "return".
 Definition noreturnV: val := #str "noreturn".
@@ -47,5 +37,88 @@ Proof.
   unfold code_block.
   wp_pures.
 Abort.
+
+Axiom eval_exprs_unordered : list (expr) → expr.
+
+Definition f : val :=
+  λ: <>, #3.
+
+Definition g : val :=
+  λ: <>, #5.
+
+Definition h : val :=
+  λ: <>, #7.
+
+(* y[f()] = g(z || h(), i()+x[j()], <-c) *)
+Definition order_of_eval_test : val :=
+  λ: <>,
+  let: "x" := (eval_exprs_unordered [f #(); g #(); h#()]) in
+  Fst "x"
+.
+
+Definition sp e P : val → iProp Σ :=
+  λ v, (∀ Φ, (P -∗ WP e {{ Φ }}) -∗ Φ v)%I.
+
+Axiom wp_eval_exprs_unordered3 :
+  ∀ e1 e2 e3 Φ1 Φ2 Φ3 (Φ:_ → iProp Σ),
+  (WP e1 {{ Φ1 }} ∗
+  WP e3 {{ Φ2 }} ∗
+  WP e3 {{ Φ3 }} ∗
+  (∀ v1 v2 v3, Φ1 v1 ∗ Φ2 v2 ∗ Φ3 v3 -∗ (Φ (v1, (v2, v3))%V))) -∗
+  WP (eval_exprs_unordered [e1 ; e2 ; e3]) {{ Φ }}
+.
+
+(*
+Axiom wp_sp_eval_exprs_unordered3 :
+  ∀ e1 e2 e3 (Φ:_ → iProp Σ),
+  (sp e1 Φ1∗
+  sp e3 Φ2 ∗
+  WP e3 {{ Φ3 }} ∗
+  (∀ v  -∗ (Φ (v1, (v2, v3))%V))) -∗
+  WP (eval_exprs_unordered [e1 ; e2 ; e3]) {{ Φ }}
+. *)
+
+Lemma wp_value (v:val) :
+  ⊢ WP of_val v {{ v', ⌜ v' = v ⌝ }}.
+Proof. by iApply wp_value. Qed.
+
+Lemma wp_order_of_eval_test :
+  ∀ Φ,
+  Φ #3 -∗
+  WP order_of_eval_test #() {{ Φ }}
+.
+Proof.
+  iIntros (?) "HΦ".
+  wp_lam.
+  wp_apply wp_eval_exprs_unordered3.
+  iSplitR.
+  (* FIXME: is there a setup where it is not necessary to have this explicit
+     intermediate predicate? *)
+  {
+    unfold f.
+    (* wp_pures without wp_finish *)
+    lazymatch goal with
+    | |- envs_entails ?envs (wp ?s ?E ?e ?Q) =>
+        let e := eval simpl in e in
+          reshape_expr e ltac:(fun K e' =>
+                                 wp_pure_filter e';
+                                 eapply (tac_wp_pure_no_later _ _ _ K e')
+                              ) || fail "wp_pure: cannot find redex pattern"
+    | _ => fail "wp_pure: not a 'wp'"
+    end.
+    { apply _. }
+    { done. }
+    simpl.
+    iApply wp_value.
+  }
+  iSplitR.
+  { wp_lam. instantiate (1:=(λ v, ⌜v = #_⌝)%I). done. }
+  iSplitR.
+  { wp_lam. instantiate (1:=(λ v, ⌜v = #_⌝)%I). done. }
+  iIntros "* (%&%&%)".
+  subst.
+  wp_pures.
+  by iApply "HΦ".
+Qed.
 
 End proof.
